{
 "cells": [
  {
   "cell_type": "code",
   "execution_count": 15,
   "id": "8228bd04-b98e-4aea-823a-122166351983",
   "metadata": {},
   "outputs": [],
   "source": [
    "# Authored by Lele Liu (2023)\n",
    "# Code for the paper -- Extremal spectral radius of nonregular graphs with prescribed maximum degree\n",
    "#\n",
    "# Code for Case 2 in the proof of Theorem 4.1 \n",
    "# To find f(x)\n",
    "a = SR.var('a') # a denotes x_{3k} for simplicity\n",
    "b = SR.var('b') # a denotes x_1 \n",
    "p = SR.var('p') # p denotes lambda \n",
    "#\n",
    "c = (p^2-1)*b # c denotes x_3 \n",
    "d = a*(p-1)*(p^2-p-5)/2 # d denotes x_{3k-3} \n",
    "#\n",
    "T = 2*(p^2+p-4)*(d^2-c^2)/((p-1)^2*(p-2)*(p+1)) + (2*p^4 - 16*p^3 + 11*p^2 + 50*p + 17)*a^2/4 + (2*p^2-1)*(p^2+2*p-1)*b^2/((p-1)^2)\n",
    "X = (T/(3-p)).subs(b==0).simplify_rational().collect(a)\n",
    "Y = (T/(3-p)).subs(a==0).simplify_rational().collect(b)\n",
    "#\n",
    "f = X + Y # output f(x)\n",
    "show(f)"
   ]
  },
  {
   "cell_type": "code",
   "execution_count": 17,
   "id": "be261c4b",
   "metadata": {},
   "outputs": [],
   "source": [
    "# Code for the proof of Lemma 5.1\n",
    "# To find f(x)\n",
    "a = SR.var('a')\n",
    "p = SR.var('p') # p denotes lambda for simplicity \n",
    "#\n",
    "b = a*(p-2)/2\n",
    "c = a*(p^2 - 2*p - 6)/2\n",
    "d = a*(p^3 - 3*p^2 - 5*p + 8)/4\n",
    "#\n",
    "x = a*(sqrt(2) - 1)*( -p^3 + 5*p^2 - (2-sqrt(3))*(sqrt(3)-sqrt(2))*p - 4*(sqrt(6)-1)*(sqrt(6)-sqrt(2)) )/4\n",
    "y = a*(sqrt(2) - 1)*( -p^3 + 5*p^2 + ((sqrt(2)+1)^2)*p - 4*sqrt(2) - 24 )/4 \n",
    "z = a*(sqrt(2) - 1)*( -p^3 + (7+2*sqrt(2))*p^2 - (3+4*sqrt(2))*p - 32 -12*sqrt(2) )/4 \n",
    "#\n",
    "# Y denotes the square of the norm of vector y\n",
    "Y = 1 + 4*x^2 + 2*y^2 + z^2 - 3*a^2 -2*b^2 - 2*c^2\n",
    "#\n",
    "f = (Y-1)/a^2 # output f(x)\n",
    "#\n",
    "show(f.expand().collect(p))"
   ]
  },
  {
   "cell_type": "code",
   "execution_count": 19,
   "id": "60a0d822-4a2b-4f44-80bb-139afbbf5c0d",
   "metadata": {},
   "outputs": [],
   "source": [
    "# Code for the proof of Lemma 5.2 \n",
    "# To find g(x)\n",
    "a = SR.var('a')\n",
    "p = SR.var('p') # p denotes lambda for simplicity \n",
    "b = a*(p-2)/2\n",
    "c = a*(p^2 - 2*p - 6)/2\n",
    "d = a*(p^3 - 3*p^2 - 5*p + 8)/4\n",
    "#\n",
    "x = a*( (1-sqrt(2))*p^3 + (4*sqrt(2) - 3)*p^2 + (4*sqrt(2) - sqrt(6) - 5)*p -16*sqrt(2) + 4*sqrt(6) + 8 )/4\n",
    "y = a*( (1-sqrt(2))*p^3 + (4*sqrt(2) - 3)*p^2 + (4*sqrt(2) - 5)*p - 16*sqrt(2) + 8 )/4\n",
    "z = a*( (1-sqrt(2))*p^3 + (5*sqrt(2) - 3)*p^2 + (sqrt(2) - 5)*p - 20*sqrt(2) + 8 )/4\n",
    "#\n",
    "# Y denote the square of the norm of vector y\n",
    "Y = 1 + 4*x^2 + 2*y^2 + 2*z^2 - (3*a^2 + 2*b^2 + 2*c^2 + d^2)\n",
    "# g(x)\n",
    "g = (Y - 1)/a^2 # output g(x)\n",
    "show(g.expand().collect(p))"
   ]
  },
  {
   "cell_type": "code",
   "execution_count": 21,
   "id": "ecc47330-0913-415c-a2b1-b4fe468429ad",
   "metadata": {},
   "outputs": [],
   "source": [
    "# Code for the proof of Lemma 5.3\n",
    "# To find h(x)\n",
    "a = SR.var('a')\n",
    "p = SR.var('p') # p denotes lambda for simplicity \n",
    "b = a*(p-3)\n",
    "c = a*(p^2 - 3*p - 2)/2\n",
    "# \n",
    "x = a*(sqrt(2) - 1)*(-p^2 + 5*p + 2*sqrt(2) - 2)/2\n",
    "y = a*(sqrt(2) - 1)*(-p^2 + (2*sqrt(2) + 7)*p - 10 - 6*sqrt(2))/2\n",
    "# Y denote the square of the norm of vector y\n",
    "Y = 1 + 4*x^2 + 3*y^2 - (4*a^2 + 2*b^2 + c^2)\n",
    "# h(x)\n",
    "h = (Y - 1)/a^2 # output h(x)\n",
    "show(h.expand().collect(p))"
   ]
  },
  {
   "cell_type": "code",
   "execution_count": 23,
   "id": "c1563c37-8c8f-4644-af26-8a676eb62eda",
   "metadata": {},
   "outputs": [],
   "source": [
    "# Code for the proof of Lemma 5.4\n",
    "a = SR.var('a')\n",
    "d = SR.var('d')\n",
    "p = SR.var('p') # p denotes lambda for simplicity\n",
    "#\n",
    "b = (2*(p - 1)*a + 4*d)/(p^2 - p - 2)\n",
    "c = 2*(a + d*p)/(p^2 - p - 2)\n",
    "x = 2*(p*a + d)/(p^2 - p - 2)\n",
    "y = (4*a + 2*(p - 1)*d)/(p^2 - p - 2)\n",
    "#\n",
    "# Compute the value of y^T L(tidle(G)) y - x^T L(G) x\n",
    "# L = y^T L(tidle(G)) y - x^T L(G) x\n",
    "L = 4*(a-x)^2 + 2*(x-y)^2 + 2*(y-d)^2 - 2*(a-b)^2 - 2*(b-c)^2 - 4*(c-d)^2\n",
    "# Compute the square of the norm of vector y\n",
    "# Y denote the square of the norm of vector y\n",
    "Y = 1 + 2*x^2 + y^2 - b^2 - 2*c^2\n",
    "#\n",
    "show(L.simplify_rational())\n",
    "show(Y.simplify_rational())"
   ]
  },
  {
   "cell_type": "code",
   "execution_count": 24,
   "id": "24be925e-0ca1-459b-8e48-5c65162b1e15",
   "metadata": {},
   "outputs": [],
   "source": [
    "# Code for the proof of Lemma 5.5\n",
    "a = SR.var('a')\n",
    "h = SR.var('h')\n",
    "p = SR.var('p') # p denotes lambda for simplicity\n",
    "#\n",
    "b = (2*(p-3)*(p+1)*a+4*h)/(p^3-2*p^2-5*p+2)\n",
    "c = (2*((p-1)*a+p*h))/(p^3-2*p^2-5*p+2)\n",
    "d = (4*a+(p-2)*(p+1)*h)/(p^3-2*p^2-5*p+2)\n",
    "#\n",
    "x = ((p-2)*(p+1)*a+4*h)/(p^3-2*p^2-5*p+2)\n",
    "y = (2*(p*a+(p-1)*h))/(p^3-2*p^2-5*p+2)\n",
    "z = (4*a+2*(p-3)*(p+1)*h)/(p^3-2*p^2-5*p+2)\n",
    "#\n",
    "# Compute the value of the right-hand side of (B.4)\n",
    "# W is the right-hand side of (B.4)\n",
    "W = (2*(a-x)^2 + 4*(x-y)^2 + 2*(y-z)^2 + 2*(z-h)^2 - 2*(a-b)^2 - 2*(b-c)^2 - 4*(c-d)^2 - 2*(d-h)^2 + 4-p)/(4-p)\n",
    "# Compute the square of the norm of vector y\n",
    "# Y denote the square of the norm of vector y\n",
    "Y = 2*x^2 + 2*y^2 + z^2 - b^2 - 2*c^2 - 2*d^2 + 1\n",
    "#  \n",
    "show(W.simplify_rational())\n",
    "show(Y.simplify_rational())"
   ]
  },
  {
   "cell_type": "code",
   "execution_count": 30,
   "id": "a26ea60c",
   "metadata": {},
   "outputs": [],
   "source": [
    "# Code for the proof of Lemma 5.6\n",
    "x = SR.var('x')\n",
    "y = SR.var('y')\n",
    "p = SR.var('p') # p denotes lambda for simplicity\n",
    "#\n",
    "a = (2*(p^3-p^2-4*p)*x + 2*(p+2)*y)/(p^4-2*p^3-5*p^2+6*p+4)\n",
    "b = (2*(2*p^2-2*p-4)*x + 2*(p^2+p-2)*y)/(p^4-2*p^3-5*p^2+6*p+4)\n",
    "c = (4*p*x + (p^3+p^2-4*p-4)*y)/(p^4-2*p^3-5*p^2+6*p+4)\n",
    "d = (8*x+2*(p^3-p^2-4*p+2)*y)/(p^4-2*p^3-5*p^2+6*p+4)\n",
    "#\n",
    "# u denotes alpha_1 for short\n",
    "u = (2*(p^3-p^2-4*p+2)*x+8*y)/(p^4-2*p^3-5*p^2+6*p+4)\n",
    "# v denotes alpha_2\n",
    "v = ((p^3+p^2-4*p-4)*x+4*p*y)/(p^4-2*p^3-5*p^2+6*p+4)\n",
    "# w denotes alpha_3\n",
    "w = ( 2*(p^2+p-2)*x + 2*(2*p^2-2*p-4)*y )/(p^4-2*p^3-5*p^2+6*p+4)\n",
    "# s denotes alpha_4\n",
    "s = ( 2*(p+2)*x + 2*(p^3-p^2-4*p)*y )/(p^4-2*p^3-5*p^2+6*p+4)\n",
    "# Compute the value of y^T L(tilde(G)) y - x^T L(G) x + 4-lambda\n",
    "# T = y^T L(tilde(G)) y - x^T L(G) x + 4-lambda\n",
    "T = 2*(x-u)^2 + 2*(x-v)^2 + 2*(u-v)^2 + 2*(v-w)^2 + 2*(w-s)^2 + 4*(s-y)^2 - 4*(x-a)^2 - 2*(a-b)^2 - 2*(b-c)^2 - 2*(c-d)^2 - 2*(c-y)^2 - 2*(d-y)^2 + 4-p\n",
    "# Compute the square of the norm of vector y\n",
    "# Y denote the square of the norm of vector y\n",
    "Y = u^2 + 2*v^2 + w^2 + 2*s^2 - 2*a^2 - b^2 - 2*c^2 - d^2 + 1\n",
    "#  \n",
    "show(T.simplify_rational().factor().collect(p)) # output the right-side hand of Equation (B.7)\n",
    "show(Y.simplify_rational()) # output Equation (B.8)"
   ]
  },
  {
   "cell_type": "code",
   "execution_count": 33,
   "id": "bca1ee8b-ee5f-46d5-b8db-556e95a63934",
   "metadata": {},
   "outputs": [],
   "source": [
    "# Code for the proof of Lemma 5.7\n",
    "a = SR.var('a')\n",
    "h = SR.var('h')\n",
    "p = SR.var('p') # p denotes lambda for simplicity\n",
    "#\n",
    "b = (2*(p^2-p-2)*a + 2*(p+2)*h)/(p*(p^2-p-4))\n",
    "c = (2*a + (p+2)*h)/(p^2-p-4)\n",
    "d = (4*a + 2*(p^2-2)*h)/(p*(p^2-p-4))\n",
    "#\n",
    "x = (2*(p^2-2)*a + 4*h)/(p*(p^2-p-4))\n",
    "y = ((p+2)*a + 2*h)/(p^2-p-4)\n",
    "z = (2*(p+2)*a + 2*(p^2-p-2)*h)/(p*(p^2-p-4))\n",
    "#\n",
    "# Compute the value of y^T L(tilde(G)) y - x^T L(G) x\n",
    "# T = y^T L(tilde(G)) y - x^T L(G) x\n",
    "T = 2*(a-x)^2 + 2*(a-y)^2 + 2*(x-y)^2 + 2*(y-z)^2 + 2*(z-h)^2 - 2*(a-b)^2 - 2*(b-c)^2 - 2*(c-d)^2 - 2*(d-h)^2 - 2*(c-h)^2\n",
    "# Compute the square of the norm of vector y\n",
    "# Y denote the square of the norm of vector y\n",
    "Y = x^2 + 2*y^2 + z^2 - b^2 - 2*c^2 - d^2 \n",
    "#\n",
    "show(T.simplify_rational().factor())\n",
    "show(Y.simplify_rational()) # output Equation (B.11)"
   ]
  }
 ],
 "metadata": {
  "kernelspec": {
   "display_name": "SageMath 10.1",
   "language": "sage",
   "name": "sagemath"
  },
  "language_info": {
   "codemirror_mode": {
    "name": "ipython",
    "version": 3
   },
   "file_extension": ".py",
   "mimetype": "text/x-python",
   "name": "python",
   "nbconvert_exporter": "python",
   "pygments_lexer": "ipython3",
   "version": "3.11.5"
  }
 },
 "nbformat": 4,
 "nbformat_minor": 5
}
